<?xml version="1.0"?>
<?xml-stylesheet type="text/xsl" href="rdfs-xhtml.xsl"?>
<rdf:RDF xmlns:skos="http://www.w3.org/2004/02/skos/core#"
         xmlns:dc="http://purl.org/dc/terms/"
         xmlns:dctype="http://purl.org/dc/dcmitype/"
         xmlns:dcat="http://www.w3.org/ns/dcat#"
         xmlns:foaf="http://xmlns.com/foaf/0.1/"
         xmlns:owl="http://www.w3.org/2002/07/owl#"
         xmlns:rdfs="http://www.w3.org/2000/01/rdf-schema#"
         xmlns:rdf="http://www.w3.org/1999/02/22-rdf-syntax-ns#">
    <owl:Ontology rdf:about="http://cldf.clld.org/terms.rdf">
        <rdfs:label xml:lang="en">The CLDF Vocabulary</rdfs:label>
        <rdfs:comment xml:lang="en">
        </rdfs:comment>
    </owl:Ontology>
    <rdf:Property rdf:about="http://cldf.clld.org/terms.rdf#alignment">
        <rdfs:isDefinedBy rdf:resource="http://cldf.clld.org/terms.rdf#"/>
        <rdfs:label xml:lang="en">Alignment</rdfs:label>
        <rdfs:comment>
            An alignment represents [segments](:cldf:Segments) which are grouped
            into a common [cognate set](:cldf:CognateSet) as a matrix in which cognate
            segments are placed in the same column while gap characters are introduced in
            those sound sequences missing a certain counterpart.
        </rdfs:comment>
        <rdfs:range rdf:resource="http://www.w3.org/2000/01/rdf-schema#Literal"/>
        <dc:source>List2014d</dc:source>
    </rdf:Property>
    <rdf:Property rdf:about="http://cldf.clld.org/terms.rdf#cognateSet">
        <rdfs:isDefinedBy rdf:resource="http://cldf.clld.org/terms.rdf#"/>
        <rdfs:label xml:lang="en">Cognate Set</rdfs:label>
        <rdfs:comment>
            An alignment represents [segments](:cldf:Segments) which are grouped
            into a common [cognate set](:cldf:CognateSet) as a matrix in which cognate
            segments are placed in the same column while gap characters are introduced in
            those sound sequences missing a certain counterpart.
        </rdfs:comment>
        <rdfs:range rdf:resource="http://www.w3.org/2000/01/rdf-schema#Literal"/>
        <dc:source>List2014d</dc:source>
    </rdf:Property>
    <rdf:Property rdf:about="http://cldf.clld.org/terms.rdf#conceptSet">
        <rdfs:isDefinedBy rdf:resource="http://cldf.clld.org/terms.rdf#"/>
        <rdfs:label xml:lang="en">Concept Set</rdfs:label>
        <rdfs:comment>
            A concept set groups a number of concept labels which are used in
            different questionnaires and were judged to denote the same concept despite
            potential differences among the concrete concept labels (be it their spelling,
            or the language in which they were originally created).
        </rdfs:comment>
        <rdfs:range rdf:resource="http://www.w3.org/2000/01/rdf-schema#Literal"/>
        <dc:source>List2016a</dc:source>
    </rdf:Property>
    <rdf:Property rdf:about="http://cldf.clld.org/terms.rdf#lexicalUnit">
        <rdfs:isDefinedBy rdf:resource="http://cldf.clld.org/terms.rdf#"/>
        <rdfs:label xml:lang="en">Lexical Unit</rdfs:label>
        <rdfs:comment>
            A lexical unit is any collection of word forms corresponding to a
            certain meaning which can be found in comparative datasets. Ideally, a lexical
            unit would just present itself as one single [form](:gold:FormUnit). However,
            in practice, scholars often list speech variants and at times even non-cognate
            alternatives for their preferred form.
        </rdfs:comment>
        <rdfs:range rdf:resource="http://www.w3.org/2000/01/rdf-schema#Literal"/>
        <dc:source></dc:source>
    </rdf:Property>
    <rdf:Property rdf:about="http://cldf.clld.org/terms.rdf#motivationStructure">
        <rdfs:isDefinedBy rdf:resource="http://cldf.clld.org/terms.rdf#"/>
        <rdfs:label xml:lang="en">Motivation Structure</rdfs:label>
        <rdfs:comment>
            The motivation structure of a word form gives glosses for each of
            its [morphemes](:gold:Morpheme). In this it is similar to an instance of
            [inter-linear-glossed text](:ref:?) which describes the underlying semantic
            motivation for a given word form. As an example, consider Chinese *shùpí*
            "bark (of a tree)" which is a compound consisting of *shù* "tree" and *pí*
            "skin", and whose motivation structure could be rendered as `tree bark`.
        </rdfs:comment>
        <rdfs:range rdf:resource="http://www.w3.org/2000/01/rdf-schema#Literal"/>
        <dc:source></dc:source>
    </rdf:Property>
    <rdf:Property rdf:about="http://cldf.clld.org/terms.rdf#prosodicStructure">
        <rdfs:isDefinedBy rdf:resource="http://cldf.clld.org/terms.rdf#"/>
        <rdfs:label xml:lang="en">prosodicStructure</rdfs:label>
        <rdfs:comment>
            The prosodic structure of a [word form](:cldf:Segments) labels
            similar prosidic contexts which may recur even withing the same word. Prosodic
            structures for a given language may have an underlying template that describes
            which syllables are possible. In Chinese dialects, for example, one could
            describe the basic template of most syllables as consisting of *initial*,
            *medial*, *nucleus*, *coda*, and *tone*, of which the nucleus and the tone as
            a suprasegmental element are usually the only required elements.
        </rdfs:comment>
        <rdfs:range rdf:resource="http://www.w3.org/2000/01/rdf-schema#Literal"/>
        <dc:source></dc:source>
    </rdf:Property>
    <rdf:Property rdf:about="http://cldf.clld.org/terms.rdf#root">
        <rdfs:isDefinedBy rdf:resource="http://cldf.clld.org/terms.rdf#"/>
        <rdfs:label xml:lang="en">root</rdfs:label>
        <rdfs:comment>
            The root of a [word form](:cldf:SoundSequence) is an abstract basic
            unit from which several [stems](:cldf:Stem) can be derived.
        </rdfs:comment>
        <rdfs:range rdf:resource="http://www.w3.org/2000/01/rdf-schema#Literal"/>
        <dc:source></dc:source>
    </rdf:Property>
    <rdf:Property rdf:about="http://cldf.clld.org/terms.rdf#stem">
        <rdfs:isDefinedBy rdf:resource="http://cldf.clld.org/terms.rdf#"/>
        <rdfs:label xml:lang="en">stem</rdfs:label>
        <rdfs:comment>
            A stem is a concrete [word form](:cldf:SoundSequence) in a language
            which has been derived as such from a given [root](:cldf:Root).
        </rdfs:comment>
        <rdfs:range rdf:resource="http://www.w3.org/2000/01/rdf-schema#Literal"/>
        <dc:source></dc:source>
    </rdf:Property>
    <rdf:Property rdf:about="http://cldf.clld.org/terms.rdf#soundSequence">
        <rdfs:isDefinedBy rdf:resource="http://cldf.clld.org/terms.rdf#"/>
        <rdfs:label xml:lang="en">soundSequence</rdfs:label>
        <rdfs:comment>
            A sound sequence is understood as the strict segmental
            representation of a [form unit](:gold:FormUnit) of a language, which is
            usually given in phonetic transcription. [Suprasegmental
            elements](:gold:Suprasegmental), like tone or accent, of sound sequences are
            usually represented in a sequential form, although they are usually
            co-articulated along with the segmental elements of a sound sequence.
            Alternatively, suprasegmental aspects could also be represented as part of the
            [prosodic structure](:cldf:ProsodicStructure) of a word form.
        </rdfs:comment>
        <rdfs:range rdf:resource="http://www.w3.org/2000/01/rdf-schema#Literal"/>
        <dc:source></dc:source>
    </rdf:Property>
    <rdf:Property rdf:about="http://cldf.clld.org/terms.rdf#subSequence">
        <rdfs:isDefinedBy rdf:resource="http://cldf.clld.org/terms.rdf#"/>
        <rdfs:label xml:lang="en">subSequence</rdfs:label>
        <rdfs:comment>
            [Word forms](:cldf:SoundSequence) can often be subdivided into
            smaller functional units (usually corresponding to a
            [morpheme](:gold:Morpheme)). A subsequence of a sound sequence, however, does
            not necessarily need to represent a true morpheme, but rather a unit that is
            determined by scholars to serve as the basis for historical comparison.
        </rdfs:comment>
        <rdfs:range rdf:resource="http://www.w3.org/2000/01/rdf-schema#Literal"/>
        <dc:source></dc:source>
    </rdf:Property>
    <rdfs:Class rdf:about="http://cldf.clld.org/terms.rdf#Wordlist">
        <rdfs:isDefinedBy rdf:resource="http://cldf.clld.org/terms.rdf#"/>
        <rdfs:label xml:lang="en">Wordlist</rdfs:label>
        <rdfs:comment>
            A dataset according to the CLDF Wordlist specification
        </rdfs:comment>
        <rdfs:subClassOf rdf:resource="http://purl.org/dc/dcmitype/Dataset"/>
        <dc:source></dc:source>
    </rdfs:Class>
    <rdfs:Class rdf:about="http://cldf.clld.org/terms.rdf#Dictionary">
        <rdfs:isDefinedBy rdf:resource="http://cldf.clld.org/terms.rdf#"/>
        <rdfs:label xml:lang="en">Dictionary</rdfs:label>
        <rdfs:comment>
            A dataset according to the CLDF Dictionary specification
        </rdfs:comment>
        <rdfs:subClassOf rdf:resource="http://purl.org/dc/dcmitype/Dataset"/>
        <dc:source></dc:source>
    </rdfs:Class>
    <rdfs:Class rdf:about="http://cldf.clld.org/terms.rdf#StructureDataset">
        <rdfs:isDefinedBy rdf:resource="http://cldf.clld.org/terms.rdf#"/>
        <rdfs:label xml:lang="en">Structure Dataset</rdfs:label>
        <rdfs:comment>
            A dataset according to the CLDF Structure Dataset specification
        </rdfs:comment>
        <rdfs:subClassOf rdf:resource="http://purl.org/dc/dcmitype/Dataset"/>
        <dc:source></dc:source>
    </rdfs:Class>
    <rdfs:Class rdf:about="http://cldf.clld.org/terms.rdf#ValueTable">
        <rdfs:isDefinedBy rdf:resource="http://cldf.clld.org/terms.rdf#"/>
        <rdfs:label xml:lang="en">ValueTable</rdfs:label>
        <rdfs:comment></rdfs:comment>
        <dc:source></dc:source>
    </rdfs:Class>
    <rdfs:Class rdf:about="http://cldf.clld.org/terms.rdf#ExampleTable">
        <rdfs:isDefinedBy rdf:resource="http://cldf.clld.org/terms.rdf#"/>
        <rdfs:label xml:lang="en">ExampleTable</rdfs:label>
        <rdfs:comment></rdfs:comment>
        <dc:source></dc:source>
    </rdfs:Class>
    <rdfs:Class rdf:about="http://cldf.clld.org/terms.rdf#EntryTable">
        <rdfs:isDefinedBy rdf:resource="http://cldf.clld.org/terms.rdf#"/>
        <rdfs:label xml:lang="en">EntryTable</rdfs:label>
        <rdfs:comment></rdfs:comment>
        <dc:source></dc:source>
    </rdfs:Class>
    <rdfs:Class rdf:about="http://cldf.clld.org/terms.rdf#SenseTable">
        <rdfs:isDefinedBy rdf:resource="http://cldf.clld.org/terms.rdf#"/>
        <rdfs:label xml:lang="en">SenseTable</rdfs:label>
        <rdfs:comment></rdfs:comment>
        <dc:source></dc:source>
    </rdfs:Class>
    <rdfs:Class rdf:about="http://cldf.clld.org/terms.rdf#FormTable">
        <rdfs:isDefinedBy rdf:resource="http://cldf.clld.org/terms.rdf#"/>
        <rdfs:label xml:lang="en">FormTable</rdfs:label>
        <rdfs:comment></rdfs:comment>
        <dc:source></dc:source>
    </rdfs:Class>
    <rdfs:Class rdf:about="http://cldf.clld.org/terms.rdf#CognateTable">
        <rdfs:isDefinedBy rdf:resource="http://cldf.clld.org/terms.rdf#"/>
        <rdfs:label xml:lang="en">CognateTable</rdfs:label>
        <rdfs:comment></rdfs:comment>
        <dc:source></dc:source>
    </rdfs:Class>
    <rdfs:Class rdf:about="http://cldf.clld.org/terms.rdf#LanguageTable">
        <rdfs:isDefinedBy rdf:resource="http://cldf.clld.org/terms.rdf#"/>
        <rdfs:label xml:lang="en">LanguageTable</rdfs:label>
        <rdfs:comment></rdfs:comment>
        <dc:source></dc:source>
    </rdfs:Class>
</rdf:RDF>
